Smallstep.semantics: don't carry the query around
This is to make our extra LTS constructions less annoying (in particular
horizontal composition), however this means we have to embed the
relevant information in LTL, Linear and Mach states instead of using
variables a la CompCertX.

Thanksfully, this is pretty non-invasive and in fact occasionally
reduces the distance from the original Compcert.

backend/Allocproof.v
@@ -1845,10 +1845,6 @@ Proof.
   eapply function_ptr_translated; eauto.
 Qed.
 
-Section WITHINILS.
-
-Variable init_ls: locset.
-
 Lemma exec_moves:
   forall mv env rs s f sp bb m e e' ls,
   track_moves env mv e = Some e' ->
@@ -1856,7 +1852,7 @@ Lemma exec_moves:
   satisf rs ls e' ->
   wt_regset env rs ->
   exists ls',
-    star (step init_ls) tge (Block s f sp (expand_moves mv bb) ls m)
+    star step tge (Block s f sp (expand_moves mv bb) ls m)
                E0 (Block s f sp bb ls' m)
   /\ satisf rs ls' e.
 Proof.
@@ -1899,12 +1895,14 @@ Qed.
 
 (** The simulation relation *)
 
+Section WITHRESTYPE.
+Variable init_ls: locset.
 Variable restype: option typ.
 
 Inductive match_stackframes: list RTL.stackframe -> list LTL.stackframe -> signature -> Prop :=
   | match_stackframes_nil: forall sg,
-      Some sg.(sig_res) = Some restype ->
-      match_stackframes nil nil sg
+      sg.(sig_res) = restype ->
+      match_stackframes nil (Parent init_ls :: nil) sg
   | match_stackframes_cons:
       forall res f sp pc rs s tf bb ls ts sg an e env
         (STACKS: match_stackframes s ts (fn_sig tf))
@@ -1919,7 +1917,7 @@ Inductive match_stackframes: list RTL.stackframe -> list LTL.stackframe -> signa
            Val.has_type v (env res) ->
            agree_callee_save ls ls1 ->
            exists ls2,
-           star (LTL.step init_ls) tge (Block ts tf sp bb ls1 m)
+           star LTL.step tge (Block ts tf sp bb ls1 m)
                           E0 (State ts tf sp pc ls2 m)
            /\ satisf (rs#res <- v) ls2 e),
       match_stackframes
@@ -1945,7 +1943,7 @@ Inductive match_states: RTL.state -> LTL.state -> Prop :=
         (STACKS: match_stackframes s ts (funsig tf))
         (FUN: transf_fundef f = OK tf)
         (ARGS: Val.lessdef_list args (map (fun p => Locmap.getpair p ls) (loc_arguments (funsig tf))))
-        (AG: agree_callee_save (parent_locset init_ls ts) ls)
+        (AG: agree_callee_save (parent_locset ts) ls)
         (MEM: Mem.extends m m')
         (WTARGS: Val.has_type_list args (sig_args (funsig tf))),
       match_states (RTL.Callstate s f args m)
@@ -1954,7 +1952,7 @@ Inductive match_states: RTL.state -> LTL.state -> Prop :=
       forall s res m ts ls m' sg
         (STACKS: match_stackframes s ts sg)
         (RES: Val.lessdef res (Locmap.getpair (map_rpair R (loc_result sg)) ls))
-        (AG: agree_callee_save (parent_locset init_ls ts) ls)
+        (AG: agree_callee_save (parent_locset ts) ls)
         (MEM: Mem.extends m m')
         (WTRES: Val.has_type res (proj_sig_res sg)),
       match_states (RTL.Returnstate s res m)
@@ -1966,11 +1964,11 @@ Lemma match_stackframes_change_sig:
   sg'.(sig_res) = sg.(sig_res) ->
   match_stackframes s ts sg'.
 Proof.
-  intros. inv H.
+  intros. destruct H.
   constructor. congruence.
   econstructor; eauto.
   unfold proj_sig_res in *. rewrite H0; auto.
-  intros. rewrite (loc_result_exten sg' sg) in H by auto. eauto.
+  intros. rewrite (loc_result_exten sg' sg) in H1 by auto. eauto.
 Qed.
 
 Ltac UseShape :=
@@ -2001,7 +1999,7 @@ Qed.
 Lemma step_simulation:
   forall S1 t S2, RTL.step ge S1 t S2 -> wt_state restype S1 ->
   forall S1', match_states S1 S1' ->
-  exists S2', plus (LTL.step init_ls) tge S1' t S2' /\ match_states S2 S2'.
+  exists S2', plus LTL.step tge S1' t S2' /\ match_states S2 S2'.
 Proof.
   induction 1; intros WT S1' MS; inv MS; try UseShape.
 
@@ -2433,7 +2431,7 @@ Proof.
   econstructor. eauto. eauto. traceEq.
   simpl. econstructor; eauto. rewrite <- H11.
   replace (Locmap.getpair (map_rpair R (loc_result (RTL.fn_sig f)))
-                          (return_regs (parent_locset init_ls ts) ls1))
+                          (return_regs (parent_locset ts) ls1))
   with (Locmap.getpair (map_rpair R (loc_result (RTL.fn_sig f))) ls1).
   eapply add_equations_res_lessdef; eauto.
   rewrite H13. apply WTRS.
@@ -2493,7 +2491,7 @@ Proof.
   apply wt_regset_assign; auto. rewrite WTRES0; auto.
 Qed.
 
-End WITHINILS.
+End WITHRESTYPE.
 
 Let cc := cc_compose cc_extends_triangle cc_locset.
 
@@ -2516,7 +2514,7 @@ Proof.
   intros. inv H.
   exploit function_ptr_translated; eauto. intros [tf [FIND TR]].
   exploit sig_function_translated; eauto. intros SIG.
-  exists (LTL.Callstate nil tf rs m); split.
+  exists (LTL.Callstate (Parent rs :: nil) tf rs m); split.
   rewrite <- SIG.
   econstructor; eauto.
   fold tge. rewrite genv_next_preserved. assumption.
@@ -2646,7 +2644,7 @@ Proof.
 - intros. destruct H0.
   exploit step_simulation; eauto.
   intros [s2' [A B]].
-  exists s2'; split. rewrite comp_snd_q2 in A. exact A. split.
+  exists s2'; split. exact A. split.
   eapply subject_reduction; eauto. eexact wt_prog. eexact H.
   auto.
 Qed.
